ADTRefinement/BuildADTSetoidMorphisms.v
@@ -9,14 +9,14 @@ Set Implicit Arguments.
 
 Theorem refineADT_BuildADT_Rep mutSigs obsSigs oldRep newRep
       (SiR : oldRep -> newRep -> Prop)
-: respectful_hetero _ _ _ _
+: @respectful_heteroT _ _ _ _
       (fun oldMuts newMuts =>
          forall mutIdx,
            @refineMutator oldRep newRep SiR
                           _
                           (getMutDef oldMuts mutIdx)
                           (getMutDef newMuts mutIdx))
-      (fun x y => respectful_hetero _ _ _ _
+      (fun x y => @respectful_heteroT _ _ _ _
                     (fun oldObs newObs =>
                        forall obsIdx,
                          @refineObserver oldRep newRep SiR _ _
@@ -26,14 +26,31 @@ Theorem refineADT_BuildADT_Rep mutSigs obsSigs oldRep newRep
      (@BuildADT oldRep mutSigs obsSigs)
      (@BuildADT newRep mutSigs obsSigs).
  Proof.
-   unfold Proper, respectful_hetero; intros.
+   unfold Proper, respectful_heteroT; intros.
    let A := match goal with |- refineADT ?A ?B => constr:(A) end in
    let B := match goal with |- refineADT ?A ?B => constr:(B) end in
    eapply (@refinesADT _ A B SiR);
      unfold id, pointwise_relation in *; simpl in *; intros; eauto.
  Qed.
 
-Add Parametric Morphism rep mutSigs obsSigs
+Lemma refineADT_BuildADT_Both'
+      rep mutSigs obsSigs
+: forall oldMuts newMuts,
+    (forall mutIdx, @refineMutator _ _ eq _
+                                   (getMutDef oldMuts mutIdx)
+                                   (getMutDef newMuts mutIdx))
+    -> forall oldObs newObs,
+         (forall obsIdx, @refineObserver _ _ eq _ _
+                                         (getObsDef oldObs obsIdx)
+                                         (getObsDef newObs obsIdx))
+         -> refineADT (@BuildADT rep mutSigs obsSigs oldMuts oldObs)
+                      (@BuildADT rep mutSigs obsSigs newMuts newObs).
+  intros; eapply refineADT_BuildADT_Rep; eauto; reflexivity.
+Qed.
+
+Definition refineADT_BuildADT_Both := refineADT_BuildADT_Both'.
+
+(*Add Parametric Morphism rep mutSigs obsSigs
 : (@BuildADT rep mutSigs obsSigs)
     with signature
     (fun oldMuts newMuts =>
@@ -47,5 +64,5 @@ Add Parametric Morphism rep mutSigs obsSigs
       ==> refineADT
       as refineADT_BuildADT_Both.
 Proof.
-  intros; eapply refineADT_BuildADT_Rep; eauto; reflexivity.
-Qed.
+  intros; apply refineADT_BuildADT_Both'.
+Qed.*)
