ADTRefinement/GeneralBuildADTRefinements.v
@@ -159,41 +159,6 @@ Section BuildADTRefinements.
 
   Hint Resolve In_obsSigs.
 
-  Lemma refineADT_BuildADT_ReplaceObserver_generic_ex
-            (Rep : Type)
-            (mutSigs : list mutSig)
-            (obsSigs : list obsSig)
-            (mutDefs : ilist (@mutDef Rep) mutSigs)
-            (obsDefs : ilist (@obsDef Rep) obsSigs)
-            (idx : BoundedString (List.map obsID obsSigs))
-            (newDef : obsDef (nth (findIndex obsSig_eq obsSigs idx)
-                                  obsSigs ("null" : rep × () → ())%obsSig))
-            (SiR_hyp : exists SiR,
-                         (forall mutIdx,
-                            refineMutator SiR (getMutDef mutDefs mutIdx) (getMutDef mutDefs mutIdx))
-                         /\ (forall obsIdx,
-                               refineObserver SiR (getObsDef obsDefs obsIdx) (getObsDef obsDefs obsIdx))
-                         /\ refineObserver SiR
-                                           (obsBody (ith obsSig_eq obsDefs idx _
-                                                         (@Build_obsDef Rep ("null" : rep × () → ()) (fun r _ => ret tt))
-                                           ))
-                                           (obsBody newDef))
-  : refineADT
-      (BuildADT mutDefs obsDefs)
-      (ADTReplaceObsDef mutDefs obsDefs idx newDef).
-  Proof.
-    destruct SiR_hyp as [SiR [? [? ?] ] ].
-    intros; eapply refineADT_BuildADT_Rep with (SiR := SiR);
-    trivial.
-    intro obsIdx.
-    case_eq (obsSig_eq (nth (findIndex obsSig_eq obsSigs idx) obsSigs
-                            ("null" : rep × () → ())%obsSig) obsIdx);
-      intro H'.
-    - generalize (In_obsSigs_eq _ _ _ H'); intros; subst.
-      simpl; intros; erewrite ith_replace'; eauto.
-    - simpl replaceObsDef; simpl getObsDef; erewrite ith_replace; eauto.
-  Qed.
-
   Lemma refineADT_BuildADT_ReplaceObserver_generic
             (Rep : Type)
             (mutSigs : list mutSig)
@@ -217,8 +182,15 @@ Section BuildADTRefinements.
          (BuildADT mutDefs obsDefs)
          (ADTReplaceObsDef mutDefs obsDefs idx newDef).
   Proof.
-    intros.
-    eapply refineADT_BuildADT_ReplaceObserver_generic_ex; repeat (eassumption || esplit).
+    intros; eapply refineADT_BuildADT_Rep with (SiR := SiR);
+    trivial.
+    intro obsIdx.
+    case_eq (obsSig_eq (nth (findIndex obsSig_eq obsSigs idx) obsSigs
+                            ("null" : rep × () → ())%obsSig) obsIdx);
+      intro H'.
+    - generalize (In_obsSigs_eq _ _ _ H'); intros; subst.
+      simpl; intros; erewrite ith_replace'; eauto.
+    - simpl replaceObsDef; simpl getObsDef; erewrite ith_replace; eauto.
   Qed.
 
   Lemma refineADT_BuildADT_ReplaceObserver
