ADTRefinement/RefineHideADT.v
@@ -1,7 +1,34 @@
 Require Import Common Computation ADT Ensembles ADTHide.
 Require Import ADTRefinement.Core.
 
-Add Parametric Morphism
+Lemma RefineHideADT'
+      extSig'
+      oldMutatorIndex oldObserverIndex
+      (MutatorMap : oldMutatorIndex -> MutatorIndex extSig')
+      (ObserverMap : oldObserverIndex -> ObserverIndex extSig')
+      oldADT
+: forall newADT newADT',
+    refineADT newADT newADT'
+    -> arrow (refineADT oldADT (HideADT MutatorMap ObserverMap newADT))
+             (refineADT oldADT (HideADT MutatorMap ObserverMap newADT')).
+Proof.
+  unfold arrow.
+  intros ? ? [SiR ? ?] [SiR' ? ?].
+  destruct_head ADT.
+  exists (fun r_o r_n => exists r_n', SiR' r_o r_n' /\ SiR r_n' r_n);
+    simpl; intros.
+  - destruct_ex; intuition.
+    rewrite_rev_hyp; try eassumption; [].
+    autorewrite with refine_monad; f_equiv;
+    unfold pointwise_relation; intros.
+    econstructor; inversion_by computes_to_inv; eauto.
+  - destruct_ex; intuition.
+    rewrite_rev_hyp; eauto; reflexivity.
+Qed.
+
+Definition RefineHideADT := RefineHideADT'.
+
+(*Add Parametric Morphism
     extSig'
     oldMutatorIndex oldObserverIndex
     (MutatorMap : oldMutatorIndex -> MutatorIndex extSig')
@@ -12,19 +39,5 @@ Add Parametric Morphism
     refineADT ==> impl
 as RefineHideADT.
 Proof.
-  unfold impl.
-  intros; inversion H; inversion H0; subst;
-  unfold HideADT in *; destruct x; destruct y;
-  destruct oldADT; simpl in *.
-  econstructor 1 with
-  (SiR := fun r_o r_n =>
-            exists r_n', SiR0 r_o r_n' /\ SiR r_n' r_n);
-    simpl; intros.
-  - destruct_ex; intuition.
-    rewrite <- H1, <- H5; eauto.
-    autorewrite with refine_monad; f_equiv;
-    unfold pointwise_relation; intros.
-    econstructor; inversion_by computes_to_inv; eauto.
-  - destruct_ex; intuition.
-    rewrite <- H2, <- H6; eauto; reflexivity.
-Qed.
+  unfold impl; intros; apply RefineHideADT'.
+Qed.*)
