ADTRefinement/SetoidMorphisms.v
@@ -1,8 +1,8 @@
 Require Import Common Computation ADT Ensembles.
 Require Export ADTRefinement.Core.
 
-(* Definitions for integrating [refineADT] into the setoid
-   rewriting framework. *)
+(** Definitions for integrating [refineADT] into the setoid rewriting
+    framework. *)
 
 Generalizable All Variables.
 Set Implicit Arguments.
@@ -19,7 +19,7 @@ Proof.
   intro; simpl; intros; subst; reflexivity.
 Qed.
 
-Global Instance refineADT_PreOrder Sig : PreOrder (refineADT (Sig := Sig)).
+Global Instance refineADT_PreOrder Sig : PreOrderT (refineADT (Sig := Sig)).
 Proof.
   split; compute in *.
   - intro x; destruct x.
@@ -27,27 +27,28 @@ Proof.
     (SiR := @eq Rep);
       try reflexivity.
   - intros x y z H H'.
-    destruct H.
-    destruct H'; simpl in *.
+    destruct H as [SiR ? ?].
+    destruct H' as [SiR' ? ?]; simpl in *.
     econstructor 1 with
-      (SiR := fun x z => exists y, SiR x y /\ SiR0 y z);
+      (SiR := fun x z => exists y, SiR x y /\ SiR' y z);
       simpl in *; intros.
-    + destruct_ex; intuition; rewrite <- H1, <- H; eauto.
+    + destruct_ex; intuition; rewrite_rev_hyp; eauto.
       autorewrite with refine_monad; f_equiv; unfold pointwise_relation;
       intros; econstructor; inversion_by computes_to_inv;
       eauto.
-    + destruct_ex; intuition; rewrite <- H2; eauto.
+    + destruct_ex; intuition; rewrite_rev_hyp; eauto; reflexivity.
 Qed.
 
-Add Parametric Relation Sig : (ADT Sig) refineADT
+(*Add Parametric Relation Sig : (ADT Sig) refineADT
     reflexivity proved by reflexivity
     transitivity proved by transitivity
-      as refineADT_rel.
+      as refineADT_rel.*)
 
-  (* Refining the representation type is a valid refinement,
-     as long as the new methods are valid refinements.
+(** Refining the representation type is a valid refinement, as long as
+    the new methods are valid refinements.
 
-   If we had dependent setoid relations in [Type], then we could write
+    If we had dependent setoid relations in [Type], then we could
+    write
 
 <<
 Add Parametric Morphism : @Build_ADT
@@ -73,57 +74,71 @@ Qed.
     registering [Parametric Morphism]s so that it will be easy to
     integrate if dependent setoid relations are added.
 
- **)
+ *)
 
 Lemma refineADT_Build_ADT_Rep Sig oldRep newRep
       (SiR : oldRep -> newRep -> Prop)
 :
-   (respectful_hetero
-      (forall idx, mutatorMethodType oldRep (MutatorDom Sig idx))
-      (forall idx, mutatorMethodType newRep (MutatorDom Sig idx))
-      (fun oldMuts =>
-         (forall idx,
-            observerMethodType oldRep (fst (ObserverDomCod Sig idx)) (snd (ObserverDomCod Sig idx)))
-         -> ADT Sig)
-      (fun newMuts =>
-         (forall idx,
-            observerMethodType newRep (fst (ObserverDomCod Sig idx)) (snd (ObserverDomCod Sig idx)))
-         -> ADT Sig)
-      (fun oldMuts newMuts =>
-         forall mutIdx,
-           @refineMutator oldRep newRep SiR
-                          _
-                          (oldMuts mutIdx)
-                          (newMuts mutIdx))
-      (fun x y => respectful_hetero
-                    (forall idx, observerMethodType oldRep _ _)
-                    (forall idx, observerMethodType newRep _ _)
-                    (fun _ => ADT Sig)
-                    (fun _ => ADT Sig)
-                    (fun obs obs' =>
-                       forall obsIdx : ObserverIndex Sig,
-                         @refineObserver oldRep newRep SiR
-                                         (fst (ObserverDomCod Sig obsIdx))
-                                         (snd (ObserverDomCod Sig obsIdx))
+  (@respectful_heteroT
+     (forall idx, mutatorMethodType oldRep (MutatorDom Sig idx))
+     (forall idx, mutatorMethodType newRep (MutatorDom Sig idx))
+     (fun oldMuts =>
+        (forall idx,
+           observerMethodType oldRep (fst (ObserverDomCod Sig idx)) (snd (ObserverDomCod Sig idx)))
+        -> ADT Sig)
+     (fun newMuts =>
+        (forall idx,
+           observerMethodType newRep (fst (ObserverDomCod Sig idx)) (snd (ObserverDomCod Sig idx)))
+        -> ADT Sig)
+     (fun oldMuts newMuts =>
+        forall mutIdx,
+          @refineMutator oldRep newRep SiR
+                         _
+                         (oldMuts mutIdx)
+                         (newMuts mutIdx))
+     (fun x y => @respectful_heteroT
+                   (forall idx, observerMethodType oldRep _ _)
+                   (forall idx, observerMethodType newRep _ _)
+                   (fun _ => ADT Sig)
+                   (fun _ => ADT Sig)
+                   (fun obs obs' =>
+                      forall obsIdx : ObserverIndex Sig,
+                        @refineObserver oldRep newRep SiR
+                                        (fst (ObserverDomCod Sig obsIdx))
+                                        (snd (ObserverDomCod Sig obsIdx))
                                         (obs obsIdx)
                                         (obs' obsIdx))
-                    (fun obs obs' => refineADT)))
-     (@Build_ADT Sig oldRep)
-     (@Build_ADT Sig newRep).
- Proof.
-   unfold Proper, respectful_hetero; intros.
-   let A := match goal with |- refineADT ?A ?B => constr:(A) end in
-   let B := match goal with |- refineADT ?A ?B => constr:(B) end in
-   eapply (@refinesADT Sig A B SiR);
-     unfold id, pointwise_relation in *; simpl in *; intros; eauto.
- Qed.
+                   (fun obs obs' => refineADT)))
+    (@Build_ADT Sig oldRep)
+    (@Build_ADT Sig newRep).
+Proof.
+  unfold Proper, respectful_heteroT; intros.
+  let A := match goal with |- refineADT ?A ?B => constr:(A) end in
+  let B := match goal with |- refineADT ?A ?B => constr:(B) end in
+  eapply (@refinesADT Sig A B SiR);
+    unfold id, pointwise_relation in *; simpl in *; intros; eauto.
+Qed.
 
- (* Thankfully, we can register a number of different refinements
-    which follow from [refineADT_Build_ADT_Rep] as [Parametric Morphism]s. *)
+(** Thankfully, we can register a number of different refinements
+    which follow from [refineADT_Build_ADT_Rep] as [Parametric
+    Morphism]s... or we could, if [refineADT] were in [Prop]. *)
 
-(* Refining Observers is a valid ADT refinement. *)
+(** Refining Observers is a valid ADT refinement. *)
 
-Add Parametric Morphism rep Sig ms
+Lemma refineADT_Build_ADT_Observer' rep Sig ms
+: forall obs obs',
+    (forall idx, @refineObserver _ _ eq
+                                 (fst (ObserverDomCod Sig idx))
+                                 (snd (ObserverDomCod Sig idx))
+                                 (obs idx) (obs' idx))
+    -> refineADT (@Build_ADT Sig rep ms obs) (@Build_ADT Sig rep ms obs').
+Proof.
+  intros; eapply refineADT_Build_ADT_Rep; eauto; reflexivity.
+Qed.
+
+Definition refineADT_Build_ADT_Observer := refineADT_Build_ADT_Observer'.
+
+(*Add Parametric Morphism rep Sig ms
 : (@Build_ADT Sig rep ms)
     with signature
     (fun obs obs' =>
@@ -134,12 +149,23 @@ Add Parametric Morphism rep Sig ms
       ==> refineADT
       as refineADT_Build_ADT_Observer.
 Proof.
+  apply refineADT_Build_ADT_Observer'.
+Qed.*)
+
+(** Refining Mutators is also a valid ADT refinement. *)
+
+Lemma refineADT_Build_ADT_Mutators' rep Sig obs
+: forall mut mut',
+    (forall idx, @refineMutator _ _ eq
+                                (MutatorDom Sig idx)
+                                (mut idx) (mut' idx))
+    -> refineADT (@Build_ADT Sig rep mut obs) (@Build_ADT Sig rep mut' obs).
+Proof.
   intros; eapply refineADT_Build_ADT_Rep; eauto; reflexivity.
 Qed.
 
-(* Refining Mutators is also a valid ADT refinement. *)
-
-Add Parametric Morphism rep Sig obs
+Definition refineADT_Build_ADT_Mutators := refineADT_Build_ADT_Mutators'.
+(*Add Parametric Morphism rep Sig obs
 : (fun ms => @Build_ADT Sig rep ms obs)
     with signature
     (fun mut mut' =>
@@ -149,15 +175,31 @@ Add Parametric Morphism rep Sig obs
       ==> refineADT
       as refineADT_Build_ADT_Mutators.
 Proof.
+  apply refineADT_Build_ADT_Mutators'.
+Qed.*)
+
+(** Refining observers and mutators at the same time is also a valid
+    refinement. [BD: I've come to the conclusion that smaller
+    refinement steps are better, so using the previous refinements
+    should be the preferred mode. ]*)
+
+Lemma refineADT_Build_ADT_Both' rep Sig
+: forall obs obs',
+    (forall idx, @refineObserver _ _ eq
+                                 (fst (ObserverDomCod Sig idx))
+                                 (snd (ObserverDomCod Sig idx))
+                                 (obs idx) (obs' idx))
+    -> forall mut mut',
+         (forall idx, @refineMutator _ _ eq
+                                     (MutatorDom Sig idx)
+                                     (mut idx) (mut' idx))
+         -> refineADT (@Build_ADT Sig rep mut obs) (@Build_ADT Sig rep mut' obs').
+Proof.
   intros; eapply refineADT_Build_ADT_Rep; eauto; reflexivity.
 Qed.
 
-(* Refining observers and mutators at the same time is also a valid
-   refinement. [BD: I've come to the conclusion that smaller refinement
-   steps are better, so using the previous refinements should be the
-   preferred mode. ]*)
-
-Add Parametric Morphism Sig rep
+Definition refineADT_Build_ADT_Both := refineADT_Build_ADT_Both'.
+(*Add Parametric Morphism Sig rep
 : (@Build_ADT Sig rep)
     with signature
     (fun mut mut' =>
@@ -173,4 +215,4 @@ Add Parametric Morphism Sig rep
       as refineADT_Build_ADT_Both.
 Proof.
   intros; eapply refineADT_Build_ADT_Rep; eauto; reflexivity.
-Qed.
+Qed.*)
