ADTRepInv.v
@@ -3,48 +3,51 @@ Require Import Common Computation ADT Ensembles ADTRefinement.
 Generalizable All Variables.
 Set Implicit Arguments.
 
-(* Oftentimes in order to show that a refinement is valid, we
-   need some invariant to hold on an ADT's representation- a value
-   cached in an ADT's representation should be the result of running
-   an observer on the current state, for example.
+(** Oftentimes in order to show that a refinement is valid, we need
+    some invariant to hold on an ADT's representation- a value cached
+    in an ADT's representation should be the result of running an
+    observer on the current state, for example.
 
 
-   One solution to this problem is to use dependent products to package
-   proofs of an invariant into an ADT's representation: [ {rep | Invariant rep} ].
-   While conceptually simple, this forces methods to be 'internally'
-   verified- mutator methods in particular have to simultaneously produce
-   a new state /and/ a proof that it satisfies the ADT's invariant.
-   This can make derivations more painful while potentially being
-   bewildering to those unfamiliar with dependent products.
+    One solution to this problem is to use dependent products to
+    package proofs of an invariant into an ADT's representation: [
+    {rep | Invariant rep} ].
+    While conceptually simple, this forces methods to be 'internally'
+    verified- mutator methods in particular have to simultaneously
+    produce a new state /and/ a proof that it satisfies the ADT's
+    invariant.  This can make derivations more painful while
+    potentially being bewildering to those unfamiliar with dependent
+    products.
 
-   Dependent products introduce another wrinkle to refinement:
-   since an ADT refinement can change the proof produced by a method,
-   we can't always use equality as the simulation relation in
-   [ADTrefine]. (As an example of a case where the proof changes,
-   a refinement might use a cached value instead of running
-   a method on the current state.)
+    Dependent products introduce another wrinkle to refinement: since
+    an ADT refinement can change the proof produced by a method, we
+    can't always use equality as the simulation relation in
+    [ADTrefine]. (As an example of a case where the proof changes, a
+    refinement might use a cached value instead of running a method on
+    the current state.)
 
-   An alternative approach is to have the [ADT] include invariants
-   and the corresponding proofs that methods maintain them as a separate
-   fields. This more familiar presentation allows method refinements
-   to be defined and then verified interactively during a derivation,
-   at the cost of polluting ADT definitions with extra fields. Since
-   proofs aren't packaged into the representation in this approach,
-   equality suffices for expressing method refinement.
+    An alternative approach is to have the [ADT] include invariants
+    and the corresponding proofs that methods maintain them as a
+    separate fields. This more familiar presentation allows method
+    refinements to be defined and then verified interactively during a
+    derivation, at the cost of polluting ADT definitions with extra
+    fields. Since proofs aren't packaged into the representation in
+    this approach, equality suffices for expressing method refinement.
 
-   Yet another approach is to use the simulation relation to derive
-   an ad hoc invariant for a particular refinement step. The basic idea
-   is that the simulation relation relates two equal states for which
-   the invariant holds. By baking the invariant into the simulation
-   relation, it becomes a hypothesis to all of our refinement proofs.
-   The cost of this approach is that it requires a proof that each mutator
-   preserves the invariant on an ad hoc basis, which could leave to some
-   duplicate proofs (One way to mitigate this would be to include invariant
-   hypotheses around in the context, which we could bake into the honing
-   tactics). Otherwise, I [Ben] would argue it includes the best
-   of both worlds- there's no need to pollute the definition of [ADT]
-   with [repInv] /and/ methods don't have to bother with maintaining
-   proofs.
+    Yet another approach is to use the simulation relation to derive
+    an ad hoc invariant for a particular refinement step. The basic
+    idea is that the simulation relation relates two equal states for
+    which the invariant holds. By baking the invariant into the
+    simulation relation, it becomes a hypothesis to all of our
+    refinement proofs.  The cost of this approach is that it requires
+    a proof that each mutator preserves the invariant on an ad hoc
+    basis, which could leave to some duplicate proofs (One way to
+    mitigate this would be to include invariant hypotheses around in
+    the context, which we could bake into the honing
+    tactics). Otherwise, I [Ben] would argue it includes the best of
+    both worlds- there's no need to pollute the definition of [ADT]
+    with [repInv] /and/ methods don't have to bother with maintaining
+    proofs.
 
  *)
 
@@ -53,19 +56,38 @@ Section RepInv.
   Variable rep : Type.
   Variable repInv : Ensemble rep.
 
-  (* This is the simulation relation we use to mimic invariants-
-     the representations are always the same /and/ the invariant holds. *)
+  (** This is the simulation relation we use to mimic invariants- the
+      representations are always the same /and/ the invariant
+      holds. *)
 
   Definition repInvSiR (r_o r_n : rep) :=
     r_o = r_n /\ repInv r_n.
 
-  (* Refining an adt using the [repInvSiR] relation allows us to
-   utilize [repInv] when proving method refinement. Of course,
-   we also have to show that mutators preserve the invariant.
-   Hopefully we can include additional information into the honing
-   tactics to avoid reproving invariant preservation.  *)
+  (** Refining an adt using the [repInvSiR] relation allows us to
+      utilize [repInv] when proving method refinement. Of course, we
+      also have to show that mutators preserve the invariant.
+      Hopefully we can include additional information into the honing
+      tactics to avoid reproving invariant preservation.  *)
 
-  Add Parametric Morphism
+  Lemma refineADT_Build_ADT_RepInv'
+        Sig
+  : forall mut mut',
+      (forall idx, @refineMutator _ _ repInvSiR
+                                  (MutatorDom Sig idx)
+                                  (mut idx) (mut' idx))
+      -> forall obs obs',
+           (forall idx, @refineObserver _ _ repInvSiR
+                                        (fst (ObserverDomCod Sig idx))
+                                        (snd (ObserverDomCod Sig idx))
+                                        (obs idx) (obs' idx))
+           -> refineADT (@Build_ADT Sig rep mut obs)
+                        (@Build_ADT Sig rep mut' obs').
+  Proof.
+    intros; eapply refineADT_Build_ADT_Rep; eauto; reflexivity.
+  Qed.
+
+  Definition refineADT_Build_ADT_RepInv := refineADT_Build_ADT_RepInv'.
+  (*Add Parametric Morphism
       Sig
   : (@Build_ADT Sig rep)
       with signature
@@ -81,8 +103,8 @@ Section RepInv.
         ==> refineADT
         as refineADT_Build_ADT_RepInv.
   Proof.
-    intros; eapply refineADT_Build_ADT_Rep; eauto; reflexivity.
-  Qed.
+    apply refineADT_Build_ADT_RepInv'.
+  Qed.*)
 
   Lemma refine_pick_repInvSiR :
     forall r_o, repInv r_o ->
